src/Std/WP/Monad/Lemmas.lean
@@ -15,7 +15,7 @@ set_option linter.missingDocs true
 # Simp lemmas for weakest preconditions
 
 This module provides simp lemmas for simplifying weakest precondition expressions.
-Unlike `Std.Do`, we use direct function application `wp x post epost` without notation.
+Unlike `Std.Do`, we use direct function application `wp x post eposts` without notation.
 
 Some lemmas prove only one direction (`⊑`) instead of equality because our `bind_le_wp_bind` axiom
 only provides one direction.
@@ -28,147 +28,147 @@ open Lean.Order WPMonad
 universe u v
 
 section
-variable {m : Type u → Type v} [Monad m] [Assertion Pred] [Assertion EPred] [WPMonad m Pred EPred]
+variable {m : Type u → Type v} [Monad m] [Assertion Pred] [Assertion EPosts] [WPMonad m Pred EPosts]
 
 /-! ## MonadReaderOf simp lemmas -/
 
 theorem le_wp_read_ReaderT_apply
-    (post : ρ → ρ → Pred) (epost : EPred) :
-    (fun r => post r r) ⊑ wp (MonadReaderOf.read : ReaderT ρ m ρ) post epost := by
+    (post : ρ → ρ → Pred) (eposts : EPosts) :
+    (fun r => post r r) ⊑ wp (MonadReaderOf.read : ReaderT ρ m ρ) post eposts := by
   intro r
   simpa [MonadReaderOf.read] using
-    (WPMonad.pure_le_wp_pure (m := m) (x := r) (post := fun a => post a r) (epost := epost))
+    (WPMonad.pure_le_wp_pure (m := m) (x := r) (post := fun a => post a r) (eposts := eposts))
 
 @[simp]
 theorem wp_adapt_ReaderT_apply_eq (f : ρ → ρ') (x : ReaderT ρ' m α) :
-    wp (ReaderT.adapt f x : ReaderT ρ m α) post epost =
-      fun r => wp x (fun a _ => post a r) epost (f r) := rfl
+    wp (ReaderT.adapt f x : ReaderT ρ m α) post eposts =
+      fun r => wp x (fun a _ => post a r) eposts (f r) := rfl
 
 /-! ## MonadStateOf simp lemmas -/
 
 theorem le_wp_get_StateT_apply
-    (post : σ → σ → Pred) (epost : EPred) :
-    (fun s => post s s) ⊑ wp (MonadStateOf.get : StateT σ m σ) post epost := by
+    (post : σ → σ → Pred) (eposts : EPosts) :
+    (fun s => post s s) ⊑ wp (MonadStateOf.get : StateT σ m σ) post eposts := by
   intro s
   simpa [MonadStateOf.get] using!
     (WPMonad.pure_le_wp_pure (m := m) (x := (s, s))
-      (post := fun x => post x.fst x.snd) (epost := epost))
+      (post := fun x => post x.fst x.snd) (eposts := eposts))
 
 theorem le_wp_set_StateT_apply (x : σ)
-    (post : PUnit → σ → Pred) (epost : EPred) :
-    (fun _ => post ⟨⟩ x) ⊑ wp (MonadStateOf.set x : StateT σ m PUnit) post epost := by
+    (post : PUnit → σ → Pred) (eposts : EPosts) :
+    (fun _ => post ⟨⟩ x) ⊑ wp (MonadStateOf.set x : StateT σ m PUnit) post eposts := by
   intro s
   simpa [MonadStateOf.set] using!
     (WPMonad.pure_le_wp_pure (m := m) (x := (PUnit.unit, x))
-      (post := fun x => post x.fst x.snd) (epost := epost))
+      (post := fun x => post x.fst x.snd) (eposts := eposts))
 
 theorem le_wp_modifyGet_StateT_apply (f : σ → α × σ)
-    (post : α → σ → Pred) (epost : EPred) :
-    (fun s => post (f s).1 (f s).2) ⊑ wp (MonadStateOf.modifyGet f : StateT σ m α) post epost := by
+    (post : α → σ → Pred) (eposts : EPosts) :
+    (fun s => post (f s).1 (f s).2) ⊑ wp (MonadStateOf.modifyGet f : StateT σ m α) post eposts := by
   intro s
   simpa [MonadStateOf.modifyGet] using!
     (WPMonad.pure_le_wp_pure (m := m) (x := f s)
-      (post := fun x => post x.fst x.snd) (epost := epost))
+      (post := fun x => post x.fst x.snd) (eposts := eposts))
 
 theorem wp_get_EStateM_apply_eq :
-    wp (MonadStateOf.get : EStateM ε σ σ) post epost = fun s => post s s := by
+    wp (MonadStateOf.get : EStateM ε σ σ) post eposts = fun s => post s s := by
   funext s
   simp only [wp, WP.trans, MonadStateOf.get, EStateM.get]
 
 theorem wp_set_EStateM_apply_eq (x : σ) :
-    wp (MonadStateOf.set x : EStateM ε σ PUnit) post epost = fun _ => post ⟨⟩ x := by
+    wp (MonadStateOf.set x : EStateM ε σ PUnit) post eposts = fun _ => post ⟨⟩ x := by
   funext s
   simp only [wp, WP.trans, MonadStateOf.set, EStateM.set]
 
 theorem wp_modifyGet_EStateM_apply_eq (f : σ → α × σ) :
-    wp (MonadStateOf.modifyGet f : EStateM ε σ α) post epost = fun s => post (f s).1 (f s).2 := by
+    wp (MonadStateOf.modifyGet f : EStateM ε σ α) post eposts = fun s => post (f s).1 (f s).2 := by
   funext s
   simp only [wp, WP.trans, MonadStateOf.modifyGet, EStateM.modifyGet]
 
 @[simp]
 theorem wp_modify_StateT_apply_eq (f : σ → σ) :
-    wp (modify f : StateT σ m PUnit) post epost =
-      wp (MonadStateOf.modifyGet fun s => (⟨⟩, f s) : StateT σ m PUnit) post epost := by
+    wp (modify f : StateT σ m PUnit) post eposts =
+      wp (MonadStateOf.modifyGet fun s => (⟨⟩, f s) : StateT σ m PUnit) post eposts := by
   rfl
 
 @[simp]
 theorem wp_getModify_StateT_apply_eq (f : σ → σ) :
-    wp (getModify f : StateT σ m σ) post epost =
-      wp (MonadStateOf.modifyGet fun s => (s, f s) : StateT σ m σ) post epost := by
+    wp (getModify f : StateT σ m σ) post eposts =
+      wp (MonadStateOf.modifyGet fun s => (s, f s) : StateT σ m σ) post eposts := by
   rfl
 
 theorem wp_modify_EStateM_apply_eq (f : σ → σ) :
-    wp (modify f : EStateM ε σ PUnit) post epost =
-      wp (MonadStateOf.modifyGet fun s => (⟨⟩, f s) : EStateM ε σ PUnit) post epost := by
+    wp (modify f : EStateM ε σ PUnit) post eposts =
+      wp (MonadStateOf.modifyGet fun s => (⟨⟩, f s) : EStateM ε σ PUnit) post eposts := by
   rfl
 
 theorem wp_getModify_EStateM_apply_eq (f : σ → σ) :
-    wp (getModify f : EStateM ε σ σ) post epost =
-      wp (MonadStateOf.modifyGet fun s => (s, f s) : EStateM ε σ σ) post epost := by
+    wp (getModify f : EStateM ε σ σ) post eposts =
+      wp (MonadStateOf.modifyGet fun s => (s, f s) : EStateM ε σ σ) post eposts := by
   rfl
 
 /-! ## MonadExceptOf simp lemmas -/
 
 @[simp]
 theorem wp_throwThe_apply_eq [MonadExceptOf ε m] (err : ε) :
-    wp (throwThe ε err : m α) post epost =
-      wp (MonadExceptOf.throw err : m α) post epost := by
+    wp (throwThe ε err : m α) post eposts =
+      wp (MonadExceptOf.throw err : m α) post eposts := by
   rfl
 
 @[simp]
 theorem wp_throw_Except_apply_eq (e : ε) :
-    wp (MonadExceptOf.throw e : Except ε α) post epost = epost e := by
+    wp (MonadExceptOf.throw e : Except ε α) post eposts = eposts e := by
   simp [wp, WP.trans, MonadExceptOf.throw]
 
 theorem le_wp_throw_ExceptT_apply (err : ε) :
-    epost.fst err ⊑ wp (MonadExceptOf.throw err : ExceptT ε m α) post epost := by
+    eposts.fst err ⊑ wp (MonadExceptOf.throw err : ExceptT ε m α) post eposts := by
   simpa [MonadExceptOf.throw, pushExcept] using
     (WPMonad.pure_le_wp_pure (m := m) (x := Except.error err)
-      (post := pushExcept post epost.fst) (epost := epost.snd))
+      (post := pushExcept post eposts.fst) (eposts := eposts.snd))
 
 @[simp]
 theorem wp_throw_EStateM_apply_eq (e : ε) :
-    wp (MonadExceptOf.throw e : EStateM ε σ α) post epost = epost e := by
+    wp (MonadExceptOf.throw e : EStateM ε σ α) post eposts = eposts e := by
   funext s
   simp only [wp, WP.trans, MonadExceptOf.throw, EStateM.throw]
 
 @[simp]
 theorem wp_throw_Option_apply_eq (e : PUnit) :
-    wp (MonadExceptOf.throw e : Option α) post epost = epost () := by
+    wp (MonadExceptOf.throw e : Option α) post eposts = eposts () := by
   simp only [wp, MonadExceptOf.throw]
   rfl
 
 theorem le_wp_throw_OptionT_apply (err : PUnit) :
-  epost.fst () ⊑ wp (MonadExceptOf.throw err : OptionT m α) post epost := by
-  show epost.fst () ⊑ wp (pure none : m (Option α)) (pushOption post epost.fst) epost.snd
+  eposts.fst () ⊑ wp (MonadExceptOf.throw err : OptionT m α) post eposts := by
+  show eposts.fst () ⊑ wp (pure none : m (Option α)) (pushOption post eposts.fst) eposts.snd
   simpa [MonadExceptOf.throw, pushOption] using
     (WPMonad.pure_le_wp_pure (m := m) (x := none)
-      (post := pushOption post epost.fst) (epost := epost.snd))
+      (post := pushOption post eposts.fst) (eposts := eposts.snd))
 
 @[simp]
 theorem wp_tryCatch_MonadExcept_apply_eq [MonadExceptOf ε m] (x : m α)
     (h : ε → m α) :
-    wp (tryCatch x h : m α) post epost =
-      wp (MonadExceptOf.tryCatch x h : m α) post epost := by
+    wp (tryCatch x h : m α) post eposts =
+      wp (MonadExceptOf.tryCatch x h : m α) post eposts := by
   rfl
 
 @[simp]
 theorem wp_tryCatchThe_apply_eq [MonadExceptOf ε m] (x : m α) (h : ε → m α) :
-    wp (tryCatchThe ε x h : m α) post epost =
-      wp (MonadExceptOf.tryCatch x h : m α) post epost := by
+    wp (tryCatchThe ε x h : m α) post eposts =
+      wp (MonadExceptOf.tryCatch x h : m α) post eposts := by
   rfl
 
 @[simp]
 theorem wp_tryCatch_Except_apply_eq (x : Except ε α) (h : ε → Except ε α) :
-    wp (MonadExceptOf.tryCatch x h : Except ε α) post epost =
-      wp x post (fun e => wp (h e) post epost) := by
+    wp (MonadExceptOf.tryCatch x h : Except ε α) post eposts =
+      wp x post (fun e => wp (h e) post eposts) := by
   simp only [wp, WP.trans, MonadExceptOf.tryCatch, Except.tryCatch]
   cases x <;> simp
 
 theorem le_wp_tryCatch_ExceptT_apply (x : ExceptT ε m α)
     (h : ε → ExceptT ε m α) :
-    wp x post ⟨fun e => wp (h e) post epost, epost.snd⟩ ⊑
-      wp (MonadExceptOf.tryCatch x h : ExceptT ε m α) post epost := by
+    wp x post ⟨fun e => wp (h e) post eposts, eposts.snd⟩ ⊑
+      wp (MonadExceptOf.tryCatch x h : ExceptT ε m α) post eposts := by
   change _ ⊑ wp (tryCatch x h : ExceptT ε m α) _ _
   simp only [ExceptT.wp_apply_eq, ExceptT.run_tryCatch]
   apply PartialOrder.rel_trans; rotate_left; apply WPMonad.bind_le_wp_bind
@@ -180,15 +180,15 @@ theorem le_wp_tryCatch_ExceptT_apply (x : ExceptT ε m α)
 
 @[simp]
 theorem wp_tryCatch_Option_apply_eq (x : Option α) (h : PUnit → Option α) :
-  wp (MonadExceptOf.tryCatch x h : Option α) post epost =
-    wp x post (fun _ => wp (h ⟨⟩) post epost) := by
+  wp (MonadExceptOf.tryCatch x h : Option α) post eposts =
+    wp x post (fun _ => wp (h ⟨⟩) post eposts) := by
   simp only [wp, WP.trans, MonadExceptOf.tryCatch, Option.tryCatch]
   cases x <;> rfl
 
 
 theorem wp_tryCatch_EStateM_apply_eq (x : EStateM ε σ α) (h : ε → EStateM ε σ α) :
-    wp (MonadExceptOf.tryCatch x h : EStateM ε σ α) post epost =
-      fun s => wp x post (fun e s' => wp (h e) post epost s') s := by
+    wp (MonadExceptOf.tryCatch x h : EStateM ε σ α) post eposts =
+      fun s => wp x post (fun e s' => wp (h e) post eposts s') s := by
   funext s
   simp only [wp, WP.trans, MonadExceptOf.tryCatch, EStateM.tryCatch]
   cases (x s) <;> simp
@@ -197,8 +197,8 @@ theorem wp_tryCatch_EStateM_apply_eq (x : EStateM ε σ α) (h : ε → EStateM 
 @[simp]
 theorem le_wp_tryCatch_OptionT_apply (x : OptionT m α)
     (h : PUnit → OptionT m α) :
-  wp x post ⟨fun _ => wp (h ⟨⟩) post epost, epost.snd⟩ ⊑
-    wp (MonadExceptOf.tryCatch x h : OptionT m α) post epost := by
+  wp x post ⟨fun _ => wp (h ⟨⟩) post eposts, eposts.snd⟩ ⊑
+    wp (MonadExceptOf.tryCatch x h : OptionT m α) post eposts := by
   simp only [wp, MonadExceptOf.tryCatch, OptionT.tryCatch, OptionT.mk]
   apply PartialOrder.rel_trans; rotate_left; apply WPMonad.bind_le_wp_bind
   apply WP.wp_monotone_post (x := x.run); intro o; cases o with
@@ -211,75 +211,75 @@ theorem le_wp_tryCatch_OptionT_apply (x : OptionT m α)
 
 @[simp]
 theorem wp_getThe_StateT_apply_eq :
-    wp (getThe σ : StateT σ m σ) post epost =
-      wp (MonadStateOf.get : StateT σ m σ) post epost := by
+    wp (getThe σ : StateT σ m σ) post eposts =
+      wp (MonadStateOf.get : StateT σ m σ) post eposts := by
   rfl
 
 @[simp]
 theorem wp_modifyThe_StateT_apply_eq (f : σ → σ) :
-    wp (modifyThe σ f : StateT σ m PUnit) post epost =
-      wp (MonadStateOf.modifyGet fun s => (⟨⟩, f s) : StateT σ m PUnit) post epost := by
+    wp (modifyThe σ f : StateT σ m PUnit) post eposts =
+      wp (MonadStateOf.modifyGet fun s => (⟨⟩, f s) : StateT σ m PUnit) post eposts := by
   rfl
 
 @[simp]
 theorem wp_modifyGetThe_StateT_apply_eq (f : σ → α × σ) :
-    wp (modifyGetThe σ f : StateT σ m α) post epost =
-      wp (MonadStateOf.modifyGet f : StateT σ m α) post epost := by
+    wp (modifyGetThe σ f : StateT σ m α) post eposts =
+      wp (MonadStateOf.modifyGet f : StateT σ m α) post eposts := by
   rfl
 
 @[simp]
 theorem wp_get_MonadState_apply_eq [MonadStateOf σ m] :
-    wp (MonadState.get : m σ) post epost =
-      wp (MonadStateOf.get : m σ) post epost := by
+    wp (MonadState.get : m σ) post eposts =
+      wp (MonadStateOf.get : m σ) post eposts := by
   rfl
 
 @[simp]
 theorem wp_set_MonadState_apply_eq [MonadStateOf σ m] (x : σ) :
-    wp (MonadState.set x : m PUnit) post epost =
-      wp (MonadStateOf.set x : m PUnit) post epost := by
+    wp (MonadState.set x : m PUnit) post eposts =
+      wp (MonadStateOf.set x : m PUnit) post eposts := by
   rfl
 
 @[simp]
 theorem wp_modifyGet_MonadState_apply_eq [MonadStateOf σ m] (f : σ → α × σ) :
-    wp (MonadState.modifyGet f : m α) post epost =
-      wp (MonadStateOf.modifyGet f : m α) post epost := by
+    wp (MonadState.modifyGet f : m α) post eposts =
+      wp (MonadStateOf.modifyGet f : m α) post eposts := by
   rfl
 
 @[simp]
 theorem wp_read_MonadReader_apply_eq [MonadReaderOf ρ m] :
-    wp (MonadReader.read : m ρ) post epost =
-      wp (MonadReaderOf.read : m ρ) post epost := by
+    wp (MonadReader.read : m ρ) post eposts =
+      wp (MonadReaderOf.read : m ρ) post eposts := by
   rfl
 
 @[simp]
 theorem wp_readThe_ReaderT_apply_eq :
-    wp (readThe ρ : ReaderT ρ m ρ) post epost =
-      wp (MonadReaderOf.read : ReaderT ρ m ρ) post epost := by
+    wp (readThe ρ : ReaderT ρ m ρ) post eposts =
+      wp (MonadReaderOf.read : ReaderT ρ m ρ) post eposts := by
   rfl
 
 /-! ## MonadLift simp lemmas -/
 
 theorem le_wp_monadLift_StateT_apply (x : m α) (post : α → σ → Pred) :
-    (fun s => wp x (fun a => post a s) epost) ⊑
-      wp (MonadLift.monadLift x : StateT σ m α) post epost := by
+    (fun s => wp x (fun a => post a s) eposts) ⊑
+      wp (MonadLift.monadLift x : StateT σ m α) post eposts := by
   intro s
   simp only [wp, MonadLift.monadLift]
   apply PartialOrder.rel_trans; rotate_left; apply WPMonad.bind_le_wp_bind
   apply WP.wp_monotone_post; intro a
   simpa using
     (WPMonad.pure_le_wp_pure (m := m) (x := (a, s))
-      (post := fun x => post x.fst x.snd) (epost := epost))
+      (post := fun x => post x.fst x.snd) (eposts := eposts))
 
 @[simp]
 theorem wp_monadLift_ReaderT_apply_eq (x : m α) :
-    wp (MonadLift.monadLift x : ReaderT ρ m α) post epost =
-      fun r => wp x (fun a => post a r) epost := by
+    wp (MonadLift.monadLift x : ReaderT ρ m α) post eposts =
+      fun r => wp x (fun a => post a r) eposts := by
   rfl
 
 theorem le_wp_monadLift_ExceptT_apply (x : m α) (post : α → Pred)
-    (epost : (ε → Pred) × EPred) :
-    wp x post epost.snd ⊑
-      wp (MonadLift.monadLift x : ExceptT ε m α) post epost := by
+    (eposts : (ε → Pred) × EPosts) :
+    wp x post eposts.snd ⊑
+      wp (MonadLift.monadLift x : ExceptT ε m α) post eposts := by
   simp only [wp, MonadLift.monadLift, ExceptT.lift, ExceptT.mk]
   apply PartialOrder.rel_trans; rotate_left
   · exact WPMonad.map_le_wp_map (m := m) Except.ok x _ _
@@ -287,20 +287,20 @@ theorem le_wp_monadLift_ExceptT_apply (x : m α) (post : α → Pred)
 
 @[simp]
 theorem wp_lift_StateT_apply_eq (x : m α) :
-    wp (StateT.lift x : StateT σ m α) post epost =
-      wp (MonadLift.monadLift x : StateT σ m α) post epost := by
+    wp (StateT.lift x : StateT σ m α) post eposts =
+      wp (MonadLift.monadLift x : StateT σ m α) post eposts := by
   rfl
 
 @[simp]
 theorem wp_lift_ExceptT_apply_eq (x : m α) :
-    wp (ExceptT.lift x : ExceptT ε m α) post epost =
-      wp (MonadLift.monadLift x : ExceptT ε m α) post epost := by
+    wp (ExceptT.lift x : ExceptT ε m α) post eposts =
+      wp (MonadLift.monadLift x : ExceptT ε m α) post eposts := by
   rfl
 
 @[simp]
 theorem le_wp_monadLift_OptionT_apply (x : m α) :
-  wp x post epost.snd ⊑
-    wp (MonadLift.monadLift x : OptionT m α) post epost := by
+  wp x post eposts.snd ⊑
+    wp (MonadLift.monadLift x : OptionT m α) post eposts := by
   simp only [wp, MonadLift.monadLift, OptionT.mk, OptionT.lift]
   apply PartialOrder.rel_trans; rotate_left; apply WPMonad.bind_le_wp_bind
   apply WP.wp_monotone_post; intro a
@@ -309,63 +309,63 @@ theorem le_wp_monadLift_OptionT_apply (x : m α) :
 
 @[simp]
 theorem wp_lift_OptionT_apply_eq (x : m α) :
-    wp (OptionT.lift x : OptionT m α) post epost =
-      wp (MonadLift.monadLift x : OptionT m α) post epost := rfl
+    wp (OptionT.lift x : OptionT m α) post eposts =
+      wp (MonadLift.monadLift x : OptionT m α) post eposts := rfl
 
 /-! ## MonadFunctor simp lemmas -/
 
 @[simp]
 theorem wp_monadMap_StateT_apply_eq
-    (f : ∀{β}, m β → m β) {α} (x : StateT σ m α) (post : α → σ → Pred) (epost : EPred) :
-    wp (MonadFunctor.monadMap (m:=m) f x : StateT σ m α) post epost =
-      fun s => wp (f (x.run s)) (fun (a, s') => post a s') epost := by
+    (f : ∀{β}, m β → m β) {α} (x : StateT σ m α) (post : α → σ → Pred) (eposts : EPosts) :
+    wp (MonadFunctor.monadMap (m:=m) f x : StateT σ m α) post eposts =
+      fun s => wp (f (x.run s)) (fun (a, s') => post a s') eposts := by
   funext s
   simp [MonadFunctor.monadMap, StateT.run]
 
 @[simp]
 theorem wp_monadMap_ReaderT_apply_eq
-    (f : ∀{β}, m β → m β) {α} (x : ReaderT ρ m α) (post : α → ρ → Pred) (epost : EPred) :
-    wp (MonadFunctor.monadMap (m:=m) f x : ReaderT ρ m α) post epost =
-      fun r => wp (f (x.run r)) (fun a => post a r) epost := by
+    (f : ∀{β}, m β → m β) {α} (x : ReaderT ρ m α) (post : α → ρ → Pred) (eposts : EPosts) :
+    wp (MonadFunctor.monadMap (m:=m) f x : ReaderT ρ m α) post eposts =
+      fun r => wp (f (x.run r)) (fun a => post a r) eposts := by
   funext r
   simp [MonadFunctor.monadMap, ReaderT.run]
 
 @[simp]
 theorem wp_monadMap_ExceptT_apply_eq
     (f : ∀{β}, m β → m β) {α} (x : ExceptT ε m α) (post : α → Pred)
-    (epost : (ε → Pred) × EPred) :
-    wp (MonadFunctor.monadMap (m:=m) f x : ExceptT ε m α) post epost =
-      wp (f x.run) (pushExcept post epost.fst) epost.snd := by
+    (eposts : (ε → Pred) × EPosts) :
+    wp (MonadFunctor.monadMap (m:=m) f x : ExceptT ε m α) post eposts =
+      wp (f x.run) (pushExcept post eposts.fst) eposts.snd := by
   simp [MonadFunctor.monadMap, ExceptT.run]
 
 @[simp]
 theorem wp_monadMap_OptionT_apply_eq
-  (f : ∀{β}, m β → m β) {α} (x : OptionT m α) (post : α → Pred) (epost : (Unit → Pred) × EPred) :
-  wp (MonadFunctor.monadMap (m:=m) f x : OptionT m α) post epost =
-    wp (f x.run) (pushOption post epost.fst) epost.snd := by
+  (f : ∀{β}, m β → m β) {α} (x : OptionT m α) (post : α → Pred) (eposts : (Unit → Pred) × EPosts) :
+  wp (MonadFunctor.monadMap (m:=m) f x : OptionT m α) post eposts =
+    wp (f x.run) (pushOption post eposts.fst) eposts.snd := by
   simp only [wp, MonadFunctor.monadMap, OptionT.run]; rfl
 
 @[simp]
 theorem wp_withReader_ReaderT_apply_eq (f : ρ → ρ) (x : ReaderT ρ m α) :
-    wp (MonadWithReaderOf.withReader f x : ReaderT ρ m α) post epost =
-      fun r => wp x (fun a _ => post a r) epost (f r) := rfl
+    wp (MonadWithReaderOf.withReader f x : ReaderT ρ m α) post eposts =
+      fun r => wp x (fun a _ => post a r) eposts (f r) := rfl
 
 @[simp]
 theorem wp_withReader_MonadWithReader_apply_eq [MonadWithReaderOf ρ m]
     (f : ρ → ρ) (x : m α) :
-    wp (MonadWithReader.withReader f x : m α) post epost =
-      wp (MonadWithReaderOf.withReader f x : m α) post epost := rfl
+    wp (MonadWithReader.withReader f x : m α) post eposts =
+      wp (MonadWithReaderOf.withReader f x : m α) post eposts := rfl
 
 @[simp]
 theorem wp_withTheReader_ReaderT_apply_eq (f : ρ → ρ) (x : ReaderT ρ m α) :
-    wp (withTheReader ρ f x : ReaderT ρ m α) post epost =
-      wp (MonadWithReaderOf.withReader f x : ReaderT ρ m α) post epost := rfl
+    wp (withTheReader ρ f x : ReaderT ρ m α) post eposts =
+      wp (MonadWithReaderOf.withReader f x : ReaderT ρ m α) post eposts := rfl
 
 /-! ## Transformer adapt lemmas -/
 
 theorem le_wp_adapt_ExceptT_apply (f : ε → ε') (x : ExceptT ε m α) :
-    wp x post ⟨fun e => epost.fst (f e), epost.snd⟩ ⊑
-      wp (ExceptT.adapt f x : ExceptT ε' m α) post epost := by
+    wp x post ⟨fun e => eposts.fst (f e), eposts.snd⟩ ⊑
+      wp (ExceptT.adapt f x : ExceptT ε' m α) post eposts := by
   simp only [wp, ExceptT.adapt, ExceptT.mk]
   apply PartialOrder.rel_trans; rotate_left
   · exact WPMonad.map_le_wp_map (m := m) (Except.mapError f) x _ _
@@ -373,8 +373,8 @@ theorem le_wp_adapt_ExceptT_apply (f : ε → ε') (x : ExceptT ε m α) :
 
 @[simp]
 theorem wp_adaptExcept_EStateM_apply_eq (f : ε → ε') (x : EStateM ε σ α) :
-    wp (EStateM.adaptExcept f x : EStateM ε' σ α) post epost =
-      wp x post (fun e => epost (f e)) := by
+    wp (EStateM.adaptExcept f x : EStateM ε' σ α) post eposts =
+      wp x post (fun e => eposts (f e)) := by
   funext s
   simp only [wp, WP.trans, EStateM.adaptExcept]
   cases (x s) <;> simp
@@ -384,37 +384,37 @@ theorem wp_adaptExcept_EStateM_apply_eq (f : ε → ε') (x : EStateM ε σ α) 
 @[simp]
 theorem wp_liftWith_StateT_apply_eq
     (f : (∀{β}, StateT σ m β → m (β × σ)) → m α) :
-    wp (MonadControl.liftWith (m:=m) f : StateT σ m α) post epost s =
-      wp ((fun a => (a, s)) <$> f (fun x => x.run s)) (fun ⟨a, s⟩ => post a s) epost := by
+    wp (MonadControl.liftWith (m:=m) f : StateT σ m α) post eposts s =
+      wp ((fun a => (a, s)) <$> f (fun x => x.run s)) (fun ⟨a, s⟩ => post a s) eposts := by
   simp [MonadControl.liftWith]
 
 @[simp]
 theorem wp_liftWith_ReaderT_apply_eq
     (f : (∀{β}, ReaderT ρ m β → m β) → m α) :
-    wp (MonadControl.liftWith (m:=m) f : ReaderT ρ m α) post epost r =
-      wp (f (fun x => x.run r)) (fun a => post a r) epost := by
+    wp (MonadControl.liftWith (m:=m) f : ReaderT ρ m α) post eposts r =
+      wp (f (fun x => x.run r)) (fun a => post a r) eposts := by
   simp [MonadControl.liftWith, ReaderT.run]
 
 @[simp]
 theorem wp_liftWith_ExceptT_apply_eq
     (f : (∀{β}, ExceptT ε m β → m (Except ε β)) → m α) :
-    wp (MonadControl.liftWith (m:=m) f : ExceptT ε m α) post epost =
-      wp (Except.ok <$> f (fun x => x.run)) (pushExcept post epost.fst) epost.snd := by
-  change wp (liftWith (m:=m) f : ExceptT ε m α) post epost =
-    wp (Except.ok <$> f (fun x => x.run)) (pushExcept post epost.fst) epost.snd
+    wp (MonadControl.liftWith (m:=m) f : ExceptT ε m α) post eposts =
+      wp (Except.ok <$> f (fun x => x.run)) (pushExcept post eposts.fst) eposts.snd := by
+  change wp (liftWith (m:=m) f : ExceptT ε m α) post eposts =
+    wp (Except.ok <$> f (fun x => x.run)) (pushExcept post eposts.fst) eposts.snd
   simp
 
 @[simp]
 theorem le_wp_liftWith_OptionT_apply
   (f : (∀{β}, OptionT m β → m (Option β)) → m α) :
-  wp (f (fun x => x.run)) post epost.snd ⊑
-    wp (MonadControl.liftWith (m:=m) f : OptionT m α) post epost := by
+  wp (f (fun x => x.run)) post eposts.snd ⊑
+    wp (MonadControl.liftWith (m:=m) f : OptionT m α) post eposts := by
   simp only [MonadControl.liftWith, liftM, monadLift, OptionT.wp_apply_eq]
   exact le_wp_monadLift_OptionT_apply (f (fun x => x.run))
 
 theorem le_wp_restoreM_StateT_apply (x : m (α × σ)) :
-    (fun _ => wp x (fun (a, s) => post a s) epost) ⊑
-      wp (MonadControl.restoreM (m:=m) x : StateT σ m α) post epost := by
+    (fun _ => wp x (fun (a, s) => post a s) eposts) ⊑
+      wp (MonadControl.restoreM (m:=m) x : StateT σ m α) post eposts := by
   simp only [MonadControl.restoreM]
   apply PartialOrder.rel_trans; rotate_left; apply WPMonad.bind_le_wp_bind; simp only [liftM, monadLift]
   apply PartialOrder.rel_trans; rotate_left; apply le_wp_monadLift_StateT_apply
@@ -424,71 +424,71 @@ theorem le_wp_restoreM_StateT_apply (x : m (α × σ)) :
   apply PartialOrder.rel_trans
   · simpa using
       (WPMonad.pure_le_wp_pure (m := m) (x := (s'.fst, s'.snd))
-        (post := fun x => post x.fst x.snd) (epost := epost))
+        (post := fun x => post x.fst x.snd) (eposts := eposts))
   · simpa using
       (WPMonad.pure_le_wp_pure (m := m) (x := (PUnit.unit, s'.snd))
-        (post := fun (x : PUnit × σ) => wp (pure (s'.fst, x.snd)) (fun (x : α × σ) => post x.fst x.snd) epost)
-        (epost := epost))
+        (post := fun (x : PUnit × σ) => wp (pure (s'.fst, x.snd)) (fun (x : α × σ) => post x.fst x.snd) eposts)
+        (eposts := eposts))
 
 @[simp]
 theorem wp_restoreM_ReaderT_apply_eq (x : m α) :
-    wp (MonadControl.restoreM (m:=m) x : ReaderT ρ m α) post epost =
-      fun r => wp x (fun a => post a r) epost := by
+    wp (MonadControl.restoreM (m:=m) x : ReaderT ρ m α) post eposts =
+      fun r => wp x (fun a => post a r) eposts := by
   funext r
   simp [MonadControl.restoreM, ReaderT.run]
 
 @[simp]
 theorem wp_restoreM_ExceptT_apply_eq (x : m (Except ε α)) :
-    wp (MonadControl.restoreM (m:=m) x : ExceptT ε m α) post epost =
-      wp x (pushExcept post epost.fst) epost.snd := by
+    wp (MonadControl.restoreM (m:=m) x : ExceptT ε m α) post eposts =
+      wp x (pushExcept post eposts.fst) eposts.snd := by
   simp [MonadControl.restoreM, ExceptT.run]
 
 @[simp]
 theorem wp_restoreM_OptionT_apply_eq (x : m (Option α)) :
-  wp (MonadControl.restoreM (m:=m) x : OptionT m α) post epost =
-    wp x (pushOption post epost.fst) epost.snd := by
+  wp (MonadControl.restoreM (m:=m) x : OptionT m α) post eposts =
+    wp x (pushOption post eposts.fst) eposts.snd := by
   simp only [wp, MonadControl.restoreM]; rfl
 
 end
 
 @[simp]
-theorem wp_controlAt_apply_eq [Bind n] [Monad m] [Monad n] [Assertion Pred] [Assertion EPred] [∀ α, WP (n α) α Pred EPred] [MonadControlT m n]
+theorem wp_controlAt_apply_eq [Bind n] [Monad m] [Monad n] [Assertion Pred] [Assertion EPosts] [∀ α, WP (n α) α Pred EPosts] [MonadControlT m n]
     (f : (∀{β}, n β → m (stM m n β)) → m (stM m n α)) :
-    wp (controlAt m f : n α) post epost =
-      wp (liftWith f >>= restoreM : n α) post epost := by
+    wp (controlAt m f : n α) post eposts =
+      wp (liftWith f >>= restoreM : n α) post eposts := by
   rfl
 
 @[simp]
-theorem wp_control_apply_eq [Bind n] [Monad m] [Monad n] [Assertion Pred] [Assertion EPred] [∀ α, WP (n α) α Pred EPred] [MonadControlT m n]
+theorem wp_control_apply_eq [Bind n] [Monad m] [Monad n] [Assertion Pred] [Assertion EPosts] [∀ α, WP (n α) α Pred EPosts] [MonadControlT m n]
     (f : (∀{β}, n β → m (stM m n β)) → m (stM m n α)) :
-    wp (control f : n α) post epost =
-      wp (liftWith f >>= restoreM : n α) post epost := by
+    wp (control f : n α) post eposts =
+      wp (liftWith f >>= restoreM : n α) post eposts := by
   rfl
 
 section
-variable {m : Type u → Type v} [Monad m] [Assertion Pred] [Assertion EPred] [WPMonad m Pred EPred]
+variable {m : Type u → Type v} [Monad m] [Assertion Pred] [Assertion EPosts] [WPMonad m Pred EPosts]
 
 @[simp]
 theorem wp_monadLift_refl_apply_eq [Pure m] (x : m α) :
-    wp (MonadLiftT.monadLift x : m α) post epost =
-      wp (x : m α) post epost := rfl
+    wp (MonadLiftT.monadLift x : m α) post eposts =
+      wp (x : m α) post eposts := rfl
 
 @[simp]
 theorem wp_monadMap_refl_apply_eq [Pure m] (x : m α) :
-    wp (MonadFunctorT.monadMap f x : m α) post epost =
-      wp (f x : m α) post epost := by rfl
+    wp (MonadFunctorT.monadMap f x : m α) post eposts =
+      wp (f x : m α) post eposts := by rfl
 
 @[simp]
 theorem wp_liftWith_refl_apply_eq [Pure m]
     (f : (∀{β}, m β → m β) → m α) :
-    wp (MonadControlT.liftWith (m:=m) f : m α) post epost =
-      wp (f (fun x => x) : m α) post epost := by
+    wp (MonadControlT.liftWith (m:=m) f : m α) post eposts =
+      wp (f (fun x => x) : m α) post eposts := by
   rfl
 
 @[simp]
 theorem wp_restoreM_refl_apply_eq [Pure m] (x : stM m m α) :
-    wp (MonadControlT.restoreM x : m α) post epost =
-      wp (Pure.pure x : m α) post epost := by
+    wp (MonadControlT.restoreM x : m α) post eposts =
+      wp (Pure.pure x : m α) post eposts := by
   rfl
 
 end
@@ -496,34 +496,34 @@ end
 /-! ## Transitive lift/map/control simp lemmas -/
 
 section
-variable {m n : Type u → Type v} {o : Type u → Type v} [Assertion Pred] [Assertion EPred] [∀ α, WP (o α) α Pred EPred]
+variable {m n : Type u → Type v} {o : Type u → Type v} [Assertion Pred] [Assertion EPosts] [∀ α, WP (o α) α Pred EPosts]
 
 @[simp]
 theorem wp_monadLift_trans_apply_eq [MonadLift n o] [MonadLiftT m n] (x : m α) :
-    wp (MonadLiftT.monadLift x : o α) post epost =
-      wp (MonadLift.monadLift (m:=n) (MonadLiftT.monadLift (m:=m) x) : o α) post epost := rfl
+    wp (MonadLiftT.monadLift x : o α) post eposts =
+      wp (MonadLift.monadLift (m:=n) (MonadLiftT.monadLift (m:=m) x) : o α) post eposts := rfl
 
 @[simp]
 theorem wp_monadMap_trans_apply_eq [MonadFunctor n o] [MonadFunctorT m n]
     (x : o α) :
-    wp (MonadFunctorT.monadMap f x : o α) post epost =
-      wp (MonadFunctor.monadMap (m:=n) (MonadFunctorT.monadMap (m:=m) f) x : o α) post epost := by
+    wp (MonadFunctorT.monadMap f x : o α) post eposts =
+      wp (MonadFunctor.monadMap (m:=n) (MonadFunctorT.monadMap (m:=m) f) x : o α) post eposts := by
   rfl
 
 @[simp]
 theorem wp_liftWith_trans_apply_eq [MonadControl n o] [MonadControlT m n]
     (f : (∀{β}, o β → m (stM m o β)) → m α) :
-    wp (MonadControlT.liftWith f : o α) post epost =
+    wp (MonadControlT.liftWith f : o α) post eposts =
       wp (MonadControl.liftWith (m:=n) fun x₂ =>
-        MonadControlT.liftWith fun x₁ => f (x₁ ∘ x₂) : o α) post epost := by
+        MonadControlT.liftWith fun x₁ => f (x₁ ∘ x₂) : o α) post eposts := by
   rfl
 
 @[simp]
 theorem wp_restoreM_trans_apply_eq [MonadControl n o] [MonadControlT m n]
     (x : stM m o α) :
-    wp (MonadControlT.restoreM x : o α) post epost =
+    wp (MonadControlT.restoreM x : o α) post eposts =
       wp (MonadControl.restoreM (m:=n) (MonadControlT.restoreM (m:=m) x) : o α)
-        post epost := by
+        post eposts := by
   rfl
 
 end
@@ -531,30 +531,30 @@ end
 /-! ## Lifted state/reader operations -/
 
 section
-variable {m n : Type u → Type v} [MonadLift m n] [Assertion Pred] [Assertion EPred] [∀ α, WP (n α) α Pred EPred]
+variable {m n : Type u → Type v} [MonadLift m n] [Assertion Pred] [Assertion EPosts] [∀ α, WP (n α) α Pred EPosts]
 
 @[simp]
 theorem wp_get_MonadStateOf_lift_apply_eq [MonadStateOf σ m] :
-    wp (MonadStateOf.get : n σ) post epost =
-      wp (MonadLift.monadLift (MonadStateOf.get : m σ) : n σ) post epost := by
+    wp (MonadStateOf.get : n σ) post eposts =
+      wp (MonadLift.monadLift (MonadStateOf.get : m σ) : n σ) post eposts := by
   rfl
 
 @[simp]
 theorem wp_set_MonadStateOf_lift_apply_eq [MonadStateOf σ m] (x : σ) :
-    wp (MonadStateOf.set x : n PUnit) post epost =
-      wp (MonadLift.monadLift (MonadStateOf.set (σ:=σ) x : m PUnit) : n PUnit) post epost := by
+    wp (MonadStateOf.set x : n PUnit) post eposts =
+      wp (MonadLift.monadLift (MonadStateOf.set (σ:=σ) x : m PUnit) : n PUnit) post eposts := by
   rfl
 
 @[simp]
 theorem wp_modifyGet_MonadStateOf_lift_apply_eq [MonadStateOf σ m] (f : σ → α × σ) :
-    wp (MonadStateOf.modifyGet f : n α) post epost =
-      wp (MonadLift.monadLift (MonadState.modifyGet f : m α) : n α) post epost := by
+    wp (MonadStateOf.modifyGet f : n α) post eposts =
+      wp (MonadLift.monadLift (MonadState.modifyGet f : m α) : n α) post eposts := by
   rfl
 
 @[simp]
 theorem wp_read_MonadReaderOf_lift_apply_eq [MonadReaderOf ρ m] :
-    wp (MonadReaderOf.read : n ρ) post epost =
-      wp (MonadLift.monadLift (MonadReader.read : m ρ) : n ρ) post epost := by
+    wp (MonadReaderOf.read : n ρ) post eposts =
+      wp (MonadLift.monadLift (MonadReader.read : m ρ) : n ρ) post eposts := by
   rfl
 
 end
@@ -562,60 +562,60 @@ end
 /-! ## Lifted except operations -/
 
 section
-variable {m : Type u → Type v} [Monad m] [Assertion Pred] [Assertion EPred] [WPMonad m Pred EPred] [MonadExceptOf ε m]
+variable {m : Type u → Type v} [Monad m] [Assertion Pred] [Assertion EPosts] [WPMonad m Pred EPosts] [MonadExceptOf ε m]
 
 @[simp]
 theorem wp_throw_lift_ExceptT_apply_eq (err : ε) :
-    wp (MonadExceptOf.throw (ε:=ε) err : ExceptT ε' m α) post epost =
-      wp (MonadExceptOf.throw (ε:=ε) err : m (Except ε' α)) (pushExcept post epost.fst) epost.snd := by
+    wp (MonadExceptOf.throw (ε:=ε) err : ExceptT ε' m α) post eposts =
+      wp (MonadExceptOf.throw (ε:=ε) err : m (Except ε' α)) (pushExcept post eposts.fst) eposts.snd := by
   rfl
 
 @[simp]
 theorem wp_throw_lift_OptionT_apply_eq (err : ε) :
-  wp (MonadExceptOf.throw (ε:=ε) err : OptionT m α) post epost =
-    wp (MonadExceptOf.throw (ε:=ε) err : m (Option α)) (pushOption post epost.fst) epost.snd := by
+  wp (MonadExceptOf.throw (ε:=ε) err : OptionT m α) post eposts =
+    wp (MonadExceptOf.throw (ε:=ε) err : m (Option α)) (pushOption post eposts.fst) eposts.snd := by
   rfl
 
 @[simp]
 theorem wp_tryCatch_lift_ExceptT_apply_eq (x : ExceptT ε' m α) (h : ε → ExceptT ε' m α) :
-    wp (MonadExceptOf.tryCatch (ε:=ε) x h : ExceptT ε' m α) post epost =
+    wp (MonadExceptOf.tryCatch (ε:=ε) x h : ExceptT ε' m α) post eposts =
       wp (MonadExceptOf.tryCatch (ε:=ε) x h : m (Except ε' α))
-        (pushExcept post epost.fst) epost.snd := by
+        (pushExcept post eposts.fst) eposts.snd := by
   rfl
 
 @[simp]
 theorem wp_tryCatch_lift_OptionT_apply_eq (x : OptionT m α) (h : ε → OptionT m α) :
-  wp (MonadExceptOf.tryCatch (ε:=ε) x h : OptionT m α) post epost =
+  wp (MonadExceptOf.tryCatch (ε:=ε) x h : OptionT m α) post eposts =
     wp (MonadExceptOf.tryCatch (ε:=ε) x h : m (Option α))
-      (pushOption post epost.fst) epost.snd := by
+      (pushOption post eposts.fst) eposts.snd := by
   rfl
 
 @[simp]
 theorem wp_throw_ReaderT_lift_apply_eq (err : ε) :
-    wp (MonadExceptOf.throw (ε:=ε) err : ReaderT ρ m α) post epost =
+    wp (MonadExceptOf.throw (ε:=ε) err : ReaderT ρ m α) post eposts =
       wp (MonadLift.monadLift (MonadExceptOf.throw (ε:=ε) err : m α) :
-        ReaderT ρ m α) post epost := by
+        ReaderT ρ m α) post eposts := by
   rfl
 
 @[simp]
 theorem wp_throw_StateT_lift_apply_eq (err : ε) :
-    wp (MonadExceptOf.throw (ε:=ε) err : StateT σ m α) post epost =
+    wp (MonadExceptOf.throw (ε:=ε) err : StateT σ m α) post eposts =
       wp (MonadLift.monadLift (MonadExceptOf.throw (ε:=ε) err : m α) :
-        StateT σ m α) post epost := by
+        StateT σ m α) post eposts := by
   rfl
 
 @[simp]
 theorem wp_tryCatch_ReaderT_lift_apply_eq (x : ReaderT ρ m α) (h : ε → ReaderT ρ m α) :
-    wp (MonadExceptOf.tryCatch (ε:=ε) x h : ReaderT ρ m α) post epost =
+    wp (MonadExceptOf.tryCatch (ε:=ε) x h : ReaderT ρ m α) post eposts =
       fun r => wp (MonadExceptOf.tryCatch (ε:=ε) (x.run r) (fun e => (h e).run r) : m α)
-        (fun a => post a r) epost := by
+        (fun a => post a r) eposts := by
   rfl
 
 @[simp]
 theorem wp_tryCatch_StateT_lift_apply_eq (x : StateT σ m α) (h : ε → StateT σ m α) :
-    wp (MonadExceptOf.tryCatch (ε:=ε) x h : StateT σ m α) post epost =
+    wp (MonadExceptOf.tryCatch (ε:=ε) x h : StateT σ m α) post eposts =
       fun s => wp (MonadExceptOf.tryCatch (ε:=ε) (x.run s) (fun e => (h e).run s) : m (α × σ))
-        (fun (a, s') => post a s') epost := by
+        (fun (a, s') => post a s') eposts := by
   rfl
 
 end
@@ -624,25 +624,25 @@ end
 
 @[simp]
 theorem wp_orElse_Except_apply_eq (x : Except ε α) (h : Unit → Except ε α) :
-    wp (OrElse.orElse x h : Except ε α) post epost =
-      wp x post (fun _ => wp (h ()) post epost) := by
+    wp (OrElse.orElse x h : Except ε α) post eposts =
+      wp x post (fun _ => wp (h ()) post eposts) := by
   simp only [wp, OrElse.orElse, MonadExcept.orElse]
   cases x <;> rfl
 
 section
-variable {m : Type u → Type v} [Monad m] [Assertion Pred] [Assertion EPred] [WPMonad m Pred EPred]
+variable {m : Type u → Type v} [Monad m] [Assertion Pred] [Assertion EPosts] [WPMonad m Pred EPosts]
 
 theorem le_wp_orElse_ExceptT_apply (x : ExceptT ε m α)
     (h : Unit → ExceptT ε m α) :
-    wp x post ⟨fun _ => wp (h ()) post epost, epost.snd⟩ ⊑
-      wp (OrElse.orElse x h : ExceptT ε m α) post epost := by
+    wp x post ⟨fun _ => wp (h ()) post eposts, eposts.snd⟩ ⊑
+      wp (OrElse.orElse x h : ExceptT ε m α) post eposts := by
   apply le_wp_tryCatch_ExceptT_apply
 
 @[simp]
 theorem le_wp_orElse_OptionT_apply (x : OptionT m α)
     (h : Unit → OptionT m α) :
-  wp x post ⟨fun _ => wp (h ()) post epost, epost.snd⟩ ⊑
-    wp (OrElse.orElse x h : OptionT m α) post epost := by
+  wp x post ⟨fun _ => wp (h ()) post eposts, eposts.snd⟩ ⊑
+    wp (OrElse.orElse x h : OptionT m α) post eposts := by
   simp only [wp, OrElse.orElse]
   apply PartialOrder.rel_trans; rotate_left; apply WPMonad.bind_le_wp_bind
   apply WP.wp_monotone_post (x := x.run); intro o; cases o with
@@ -655,16 +655,16 @@ end
 
 @[simp]
 theorem wp_orElse_Option_apply_eq (x : Option α) (h : Unit → Option α) :
-  ∀ post (epost : Unit → Prop),
-  wp (OrElse.orElse x h : Option α) post epost =
-    wp x post (fun _ => wp (h ()) post epost) := by
+  ∀ post (eposts : Unit → Prop),
+  wp (OrElse.orElse x h : Option α) post eposts =
+    wp x post (fun _ => wp (h ()) post eposts) := by
   simp only [wp, WP.trans, OrElse.orElse, Option.orElse]
   cases x <;> intro _ _ <;> rfl
 
 @[simp]
 theorem wp_orElse_EStateM_apply_eq (x : EStateM ε σ α) (h : Unit → EStateM ε σ α) :
-    wp (OrElse.orElse x h : EStateM ε σ α) post epost =
-      fun s => wp x post (fun _ s' => wp (h ()) post epost s') s := by
+    wp (OrElse.orElse x h : EStateM ε σ α) post eposts =
+      fun s => wp x post (fun _ s' => wp (h ()) post eposts s') s := by
   funext s
   simp only [wp, WP.trans, OrElse.orElse, EStateM.orElse]
   cases x s <;> simp; rfl
