src/Std/WP/Triple/Monad.lean
@@ -23,36 +23,36 @@ The rules that build a `Triple` for `pure`, `>>=`, `<$>` and `<*>` from triples 
 namespace Std.WP
 
 universe u v w w'
-variable {Pred : Type w} {EPred : Type w'}
+variable {Pred : Type w} {EPosts : Type w'}
 
 namespace Triple
 
-variable {m : Type v → Type u} [Monad m] [Assertion Pred] [Assertion EPred]
-  [WPMonad m Pred EPred]
+variable {m : Type v → Type u} [Monad m] [Assertion Pred] [Assertion EPosts]
+  [WPMonad m Pred EPosts]
 
 theorem pure (a : α) (h : pre ⊑ post a) :
-    Triple (pure (f := m) a) pre post epost :=
-  ⟨PartialOrder.rel_trans h (WPMonad.pure_le_wp_pure a post epost)⟩
+    Triple (pure (f := m) a) pre post eposts :=
+  ⟨PartialOrder.rel_trans h (WPMonad.pure_le_wp_pure a post eposts)⟩
 
 theorem bind (x : m α) (f : α → m β)
     (mid : α → Pred)
-    (hx : Triple x pre mid epost)
-    (hf : ∀ a, Triple (f a) (mid a) post epost) :
-    Triple (x >>= f) pre post epost :=
+    (hx : Triple x pre mid eposts)
+    (hf : ∀ a, Triple (f a) (mid a) post eposts) :
+    Triple (x >>= f) pre post eposts :=
   ⟨PartialOrder.rel_trans hx.le_wp
     (PartialOrder.rel_trans
       (WP.wp_monotone_post (fun a => (hf a).le_wp))
-      (WPMonad.bind_le_wp_bind x f post epost))⟩
+      (WPMonad.bind_le_wp_bind x f post eposts))⟩
 
 theorem map [LawfulMonad m] (f : α → β) (x : m α)
-    (h : Triple x pre (fun a => post (f a)) epost) :
-    Triple (f <$> x) pre post epost :=
-  ⟨PartialOrder.rel_trans h.le_wp (WPMonad.map_le_wp_map f x post epost)⟩
+    (h : Triple x pre (fun a => post (f a)) eposts) :
+    Triple (f <$> x) pre post eposts :=
+  ⟨PartialOrder.rel_trans h.le_wp (WPMonad.map_le_wp_map f x post eposts)⟩
 
 theorem seq [LawfulMonad m] (x : m (α → β)) (y : m α)
-    (h : Triple x pre (fun f => wp y (fun a => post (f a)) epost) epost) :
-    Triple (x <*> y) pre post epost :=
-  ⟨PartialOrder.rel_trans h.le_wp (WPMonad.seq_le_wp_seq x y post epost)⟩
+    (h : Triple x pre (fun f => wp y (fun a => post (f a)) eposts) eposts) :
+    Triple (x <*> y) pre post eposts :=
+  ⟨PartialOrder.rel_trans h.le_wp (WPMonad.seq_le_wp_seq x y post eposts)⟩
 
 end Triple
 
